generalized the arc representations of corners during turning.
earlier, they were tied to wriggle. In particular, it was assumed that while turning left, the initial position was (0,0,0).
While turning right, the initial position was the position after the first move. Now, these are arbitrary

src/robots/car/exampleDimensions.v
@@ -72,6 +72,27 @@ Definition Mazda3Sedan2014sGT : CarGeometry Z := {|
   minTR := 150
 |}.
 
+Definition Mazda3Sedan2014sGTWheelsBound : CarGeometry Z := {|
+  carDim := {|
+  width := 37; (* excluding the side mirrors -- which is okay unless the curb is too high *)
+  lengthBack := 12 
+  (* radius of wheel :=
+     16/2 + 0.55*195mm converted to inches
+http://www.mycarhelpline.com/images/Tyre_Size_details.png     
+     *); 
+  lengthFront := 142;
+  |};
+  (**  To measure this, I turned the steering wheel fully left and 
+  executed a U turn in a single move, in a parking lot. During this,
+  the midpoint of the car moved sideways by 300 inches 
+  (about 2.75 parking slots, each 110 inches wide).
+  This displacement is equal to the diameter of the circle in
+  which the midpoint (of the line segment joining the rear wheels) 
+  of the car was moving.
+  *)
+  minTR := 150
+|}.
+
 Example Mazda3Sedan2014sGT_dims : 
   let cdq := (cast _ (CarDimensions Q) (Mazda3Sedan2014sGT_Dim)) in
   let trq :Z := minTR Mazda3Sedan2014sGT in
@@ -90,7 +111,36 @@ Example Mazda3Sedan2014sGT_dims :
   11= approximateAngleAsDegrees pb
   /\ 18 = approximateAngleAsDegrees mb
   /\ 9 = (( trq) - w) - R2ZApprox dex (QposMake 1 100)
-    (* 9 inches from the curb needed, else increase turn radius in second move*)
+    (* 9 inches from the curb needed, else increase turn radius in second move,
+      or don't hit the curb in first move.
+     This assumes that the curb is a wall of \inf height. 
+     Usually, the curb has much lower height (h).
+     Consider the common case where 0<h<r, where r is the radius of the wheel.
+     Then lengthBack should instead be half the length of the chord of the wheel
+     (as a circle) that is formed by intersection of the horizontal plane that denotes
+     the top surface of the curb.
+     Use the following phythagoras equation: lengthBack^2 + (r-h)^2 = r^2
+     Take the radius of the wheel as a safe approximation?
+     See below.
+      *)
+  /\ 0 = (( trq) - w) - R2ZApprox dex2 (QposMake 1 100) (* sanity check *).
+Proof using.
+  vm_compute. dands; reflexivity.
+Abort.
+
+Example Mazda3Sedan2014sGTWheelsBound_dims : 
+  let cdq := (cast _ (CarDimensions Q) (carDim Mazda3Sedan2014sGTWheelsBound)) in
+  let trq :Z := minTR Mazda3Sedan2014sGTWheelsBound in
+  let w:Z := width Mazda3Sedan2014sGT_Dim in
+  let pb :CR:= (polarTheta (transpose (βPlusBack cdq trq))) in
+  let mb :CR := (polarTheta (transpose (βMinusBack cdq trq))) in
+  let dex : CR :=  ((norm (βMinusBack cdq trq)) * (CRcos.cos (pb+mb)))%mc in
+  let dex2 : CR :=  ((norm (βMinusBack cdq trq)) * (CRcos.cos (mb)))%mc in
+  4= approximateAngleAsDegrees pb
+  /\ 6 = approximateAngleAsDegrees mb
+  /\ 1 = (( trq) - w) - R2ZApprox dex (QposMake 1 100)
+    (* 1 inches from the curb needed, else increase turn radius in second move,
+      or don't hit the curb in first move.*)
   /\ 0 = (( trq) - w) - R2ZApprox dex2 (QposMake 1 100) (* sanity check *).
 Proof using.
   vm_compute. dands; reflexivity.
